slabs bottom-up 26/n: slab selection
making progress
remaining:
- allocate_slab_aux_2
- allocate_slab
-- size class side?
- updated pack/unpack
- allocate_size_class
-- init
...

src/Slabs.fst
@@ -22,16 +22,17 @@ module SL = Selectors.LList
 //module Temp = TempLock
 
 open Utils2
+open Slots
 //open SteelOptUtils
 //open SteelStarSeqUtils
 
-let slab_region_len : U32.t = normalize_term (U32.mul page_size slab_max_number)
-unfold let slab_region
-  = r:array U8.t{A.length r = U32.v slab_region_len}
-
-let slab_md_region_len : U32.t = normalize_term (U32.mul 40ul slab_max_number)
-unfold let slab_md_region
-  = r:array U8.t{A.length r = U32.v slab_md_region_len}
+//let slab_region_len : U32.t = normalize_term (U32.mul page_size slab_max_number)
+//unfold let slab_region
+//  = r:array U8.t{A.length r = U32.v slab_region_len}
+//
+//let slab_md_region_len : U32.t = normalize_term (U32.mul 40ul slab_max_number)
+//unfold let slab_md_region
+//  = r:array U8.t{A.length r = U32.v slab_md_region_len}
 
 //// C binding, no top-level Steel initialization
 //assume val get_slab_region (_:unit)
@@ -45,57 +46,158 @@ unfold let slab_md_region
 //noextract
 //let slab_md_bitmap_length = nb_slots (U32.uint_to_t min_sc)
 
-#push-options "--print_implicits"
+#push-options "--print_implicits --print_universes"
 
 #set-options "--ide_id_info_off"
+
+noextract
+let is_empty
+  (size_class: sc)
+  (s: Seq.lseq U64.t 4)
+  : prop
+  =
+  let max = FStar.Int.max_int U64.n in
+  let bound = U32.v (nb_slots size_class) / 64 in
+  (U64.v (Seq.index s 0) = 0) /\
+  (bound > 1 && (U64.v (Seq.index s 1) = 0)) /\
+  (bound > 2 && (U64.v (Seq.index s 2) = 0)) /\
+  (bound > 3 && (U64.v (Seq.index s 3) = 0))
+
+noextract
+let is_partial
+  (size_class: sc)
+  (s: Seq.lseq U64.t 4)
+  : prop
+  =
+  ~ (is_empty size_class s) /\ has_free_slot size_class s
+
+assume val allocate_slot_refined
+  (size_class: sc)
+  (md: slab_metadata)
+  (arr: array U8.t{A.length arr = U32.v page_size})
+  : Steel (array U8.t)
+  (slab_vprop size_class arr md)
+  (fun r -> A.varray r `star` slab_vprop size_class arr md)
+  (requires fun h0 ->
+    let blob0 : (t_of (slab_vprop size_class arr md))
+      = h0 (slab_vprop size_class arr md) in
+    let v0 : Seq.lseq U64.t 4 = dfst blob0 in
+    has_free_slot size_class v0)
+  (ensures fun h0 _ h1 ->
+    let blob1 : (t_of (slab_vprop size_class arr md))
+      = h1 (slab_vprop size_class arr md) in
+    let v1 : Seq.lseq U64.t 4 = dfst blob1 in
+    is_partial size_class v1)
+
+unfold
+let blob
+  = slab_metadata &
+    (arr:array U8.t{A.length arr = U32.v page_size})
+
+//[@@__steel_reduce__]
+//unfold
+let p_empty (size_class: sc)
+  =
+  fun (b: blob) ->
+    slab_vprop size_class (snd b) (fst b)
+    `vrefine`
+    (fun (|s,_|) -> is_empty size_class s)
+
+let p_partial (size_class: sc)
+  =
+  fun (b: blob) ->
+    slab_vprop size_class (snd b) (fst b)
+    `vrefine`
+    (fun (|s,_|) -> is_partial size_class s)
+
+//#push-options "--compat_pre_typed_indexed_effects"
+//let allocate_slab_bug
+//  (sc: sc)
+//  (b: blob)
+//  : Steel unit
+//  ((slab_vprop sc (snd b) (fst b)
+//    `vrefine`
+//    (fun (|s,_|) -> is_empty sc s)))
+//  (fun _ -> (slab_vprop sc (snd b) (fst b)
+//    `vrefine`
+//    (fun (|s,_|) -> is_empty sc s)))
+//  (requires fun h0 -> True)
+//  (ensures fun _ _ _ -> True)
+//  =
+//  elim_vrefine
+//    (slab_vprop sc (snd b) (fst b))
+//    (fun (|s,_|) -> is_empty sc s);
+//  intro_vrefine
+//    (slab_vprop sc (snd b) (fst b))
+//    (fun (|s,_|) -> is_empty sc s);
+//  return ()
+//#pop-options
 
 // Given a size class, return a free slot and update metadata
 // TODO: refine spec
 // TODO: remove assume with pure predicates inside p
 //   this will yield two different versions of p
 
-(*)
+#push-options "--compat_pre_typed_indexed_effects"
+#push-options "--z3rlimit 30"
 inline_for_extraction noextract
 let allocate_slab_aux_1
   (sc: sc)
-  (partial_slabs_ptr empty_slabs_ptr: ref (SL.t slab_metadata))
-  (partial_slabs empty_slabs: SL.t slab_metadata)
+  (partial_slabs_ptr empty_slabs_ptr: ref (SL.t blob))
+  (partial_slabs empty_slabs: SL.t blob)
   : Steel (array U8.t)
-  (vptr partial_slabs_ptr `star`
-  SL.llist (p sc) partial_slabs `star`
+  (
   vptr empty_slabs_ptr `star`
-  SL.llist (p sc) empty_slabs)
-  (fun r -> SL.ind_llist (p sc) partial_slabs_ptr `star`
-  SL.ind_llist (p sc) empty_slabs_ptr)
+  SL.llist (p_empty sc) empty_slabs `star`
+  vptr partial_slabs_ptr `star`
+  SL.llist (p_partial sc) partial_slabs)
+  (fun r ->
+  A.varray r `star`
+  SL.ind_llist (p_empty sc) empty_slabs_ptr `star`
+  SL.ind_llist (p_partial sc) partial_slabs_ptr)
   (requires fun h0 ->
     sel partial_slabs_ptr h0 == partial_slabs /\
     sel empty_slabs_ptr h0 == empty_slabs /\
     not (SL.is_null_t empty_slabs))
   (ensures fun _ _ _ -> True)
   =
-  let n_empty = SL.unpack_list (p sc) empty_slabs in
-  let h = get () in
-  let md = SL.get_data n_empty in
-  assume (has_free_slot sc (A.asel md h));
-  let r = allocate_slot_kiss sc
-    (SL.get_data n_empty)
-    (f (SL.get_data n_empty)) in
+  let n_empty = SL.unpack_list (p_empty sc) empty_slabs in
+  let b = SL.get_data n_empty in
+  change_slprop_rel
+    ((p_empty sc) (SL.get_data n_empty))
+    (slab_vprop sc (snd b) (fst b)
+    `vrefine`
+    (fun (|s,_|) -> is_empty sc s))
+    (fun x y -> x == y)
+    (fun _ -> admit ());
+  elim_vrefine
+    (slab_vprop sc (snd b) (fst b))
+    (fun (|s,_|) -> is_empty sc s);
+  let r = allocate_slot_refined sc (fst b) (snd b) in
+  intro_vrefine
+    (slab_vprop sc (snd b) (fst b))
+    (fun (|s,_|) -> is_partial sc s);
+  change_slprop_rel
+    (slab_vprop sc (snd b) (fst b)
+    `vrefine`
+    (fun (|s,_|) -> is_partial sc s))
+    ((p_partial sc) (SL.get_data n_empty))
+    (fun x y -> x == y)
+    (fun _ -> admit ());
+
   let n_partial = SL.mk_cell partial_slabs (SL.get_data n_empty) in
   write empty_slabs n_partial;
-  slassert (
-    SL.llist (p sc) (SL.get_next n_empty) `star`
-    vptr empty_slabs `star`
-    (p sc) (SL.get_data n_empty)
-  );
-  SL.pack_list (p sc)
+  SL.pack_list (p_partial sc)
     empty_slabs
     partial_slabs
     (SL.get_data n_empty);
-  SL.pack_ind (p sc) empty_slabs_ptr empty_slabs;
-  write partial_slabs_ptr (SL.get_next n_empty);
-  SL.pack_ind (p sc) partial_slabs_ptr (SL.get_next n_empty);
-  return (snd r)
+  write partial_slabs_ptr empty_slabs;
+  SL.pack_ind (p_partial sc) partial_slabs_ptr empty_slabs;
+  write empty_slabs_ptr (SL.get_next n_empty);
+  SL.pack_ind (p_empty sc) empty_slabs_ptr (SL.get_next n_empty);
+  return r
 
+(*)
 inline_for_extraction noextract
 let allocate_slab_aux_2
   (sc: sc)
